feat: More supporting lemmas for OFEs (#13)

src/Iris/Algebra/OFE.lean
@@ -26,7 +26,7 @@ theorem Dist.lt [OFE α] {m n} {x y : α} : x ≡{n}≡ y → m < n → x ≡{m}
 theorem Dist.le [OFE α] {m n} {x y : α} (h : x ≡{n}≡ y) (h' : m ≤ n) : x ≡{m}≡ y :=
   if hm : m = n then hm ▸ h else h.lt (Nat.lt_of_le_of_ne h' hm)
 
-theorem Dist.rfl [OFE α] {n} {x : α} : x ≡{n}≡ x := dist_eqv.1 _
+@[simp] theorem Dist.rfl [OFE α] {n} {x : α} : x ≡{n}≡ x := dist_eqv.1 _
 theorem Dist.symm [OFE α] {n} {x : α} : x ≡{n}≡ y → y ≡{n}≡ x := dist_eqv.2
 theorem Dist.trans [OFE α] {n} {x : α} : x ≡{n}≡ y → y ≡{n}≡ z → x ≡{n}≡ z := dist_eqv.3
 
@@ -36,22 +36,24 @@ theorem equiv_eqv [ofe : OFE α] : Equivalence ofe.Equiv := by
   · rintro x y; simp [ofe.equiv_dist]; rintro h n; exact Dist.symm (h n)
   · rintro x y z; simp [ofe.equiv_dist]; rintro h₁ h₂ n; exact Dist.trans (h₁ n) (h₂ n)
 
-theorem Equiv.rfl [OFE α] {x : α} : x ≡ x := equiv_eqv.1 _
+@[simp] theorem Equiv.rfl [OFE α] {x : α} : x ≡ x := equiv_eqv.1 _
 theorem Equiv.symm [OFE α] {x : α} : x ≡ y → y ≡ x := equiv_eqv.2
 theorem Equiv.trans [OFE α] {x : α} : x ≡ y → y ≡ z → x ≡ z := equiv_eqv.3
 theorem Equiv.dist [OFE α] {x : α} : x ≡ y → x ≡{n}≡ y := (equiv_dist.1 · _)
 theorem Equiv.of_eq [OFE α] {x y : α} : x = y → x ≡ y := (· ▸ .rfl)
 
-
+/-- A function `f : α → β` is non-expansive if it preserves `n`-equivalence. -/
 class NonExpansive [OFE α] [OFE β] (f : α → β) : Prop where
   ne : ∀ ⦃n x₁ x₂⦄, x₁ ≡{n}≡ x₂ → f x₁ ≡{n}≡ f x₂
 
 instance id_ne [OFE α] : NonExpansive (@id α) := ⟨fun _ _ _ h => h⟩
 
+/-- A non-expansive function preserves equivalence. -/
 theorem NonExpansive.eqv [OFE α] [OFE β] {f : α → β} [NonExpansive f]
     ⦃x₁ x₂⦄ (h : x₁ ≡ x₂) : f x₁ ≡ f x₂ :=
   equiv_dist.2 fun _ => ne (equiv_dist.1 h _)
 
+/-- A function `f : α → β → γ` is non-expansive if it preserves `n`-equivalence in each argument. -/
 class NonExpansive₂ [OFE α] [OFE β] [OFE γ] (f : α → β → γ) : Prop where
   ne : ∀ ⦃n x₁ x₂⦄, x₁ ≡{n}≡ x₂ → ∀ ⦃y₁ y₂⦄, y₁ ≡{n}≡ y₂ → f x₁ y₁ ≡{n}≡ f x₂ y₂
 
@@ -59,40 +61,61 @@ theorem NonExpansive₂.eqv [OFE α] [OFE β] [OFE γ] {f : α → β → γ} [N
     ⦃x₁ x₂⦄ (hx : x₁ ≡ x₂) ⦃y₁ y₂⦄ (hy : y₁ ≡ y₂) : f x₁ y₁ ≡ f x₂ y₂ :=
   equiv_dist.2 fun _ => ne hx.dist hy.dist
 
+/-- `DistLater n x y` means that `x` and `y` are `m`-equivalent for all `m < n`. -/
 def DistLater [OFE α] (n : Nat) (x y : α) : Prop := ∀ m, m < n → x ≡{m}≡ y
 
-theorem DistLater.rfl [OFE α] {n} {x : α} : DistLater n x x := fun _ _ => .rfl
+@[simp] theorem DistLater.rfl [OFE α] {n} {x : α} : DistLater n x x := fun _ _ => .rfl
 theorem DistLater.symm [OFE α] {n} {x : α} (h : DistLater n x y) : DistLater n y x :=
   fun _ hm => (h _ hm).symm
 theorem DistLater.trans [OFE α] {n} {x : α} (h1 : DistLater n x y) (h2 : DistLater n y z) :
     DistLater n x z := fun _ hm => (h1 _ hm).trans (h2 _ hm)
 
+/-- `DistLater n`-equivalence is an equivalence relation. -/
 theorem distLater_eqv [OFE α] {n} : Equivalence (α := α) (DistLater n) where
   refl _ := DistLater.rfl
   symm h := h.symm
   trans h1 := h1.trans
 
+/-- `n`-equivalence implies `DistLater n`-equivalence. -/
 theorem Dist.distLater [OFE α] {n} {x y : α} (h : x ≡{n}≡ y) : DistLater n x y :=
   fun _ => dist_lt h
 
+/-- `DistLater n`-equivalence implies `m`-equivalence for all `m < n`. -/
 theorem DistLater.dist_lt [OFE α] {m n} {x y : α} (h : DistLater n x y) (hm : m < n) : x ≡{m}≡ y :=
   h _ hm
 
-theorem distLater_zero [OFE α] {x y : α} : DistLater 0 x y := nofun
+/-- `DistLater 0`-equivalence is trivial. -/
+@[simp] theorem distLater_zero [OFE α] {x y : α} : DistLater 0 x y := nofun
 
+/-- `DistLater n`-equivalence is equivalent to `(n + 1)`-equivalence. -/
 theorem distLater_succ [OFE α] {n} {x y : α} : DistLater n.succ x y ↔ x ≡{n}≡ y :=
   ⟨(·.dist_lt (Nat.lt_succ_self _)), fun h1 _ h2 => h1.le (Nat.le_of_lt_succ h2)⟩
 
+/-- A function `f : α → β` is contractive if it sends `DistLater n`-equivalent inputs to `n`-equivalent outputs. -/
 class Contractive [OFE α] [OFE β] (f : α → β) : Prop where
   distLater_dist : DistLater n x y → f x ≡{n}≡ f y
 
-theorem Contractive.zero [OFE α] [OFE β] (f : α → β) [Contractive f] {x y} : f x ≡{0}≡ f y :=
+@[simp] theorem Contractive.zero [OFE α] [OFE β] (f : α → β) [Contractive f] {x y} :
+    f x ≡{0}≡ f y :=
   Contractive.distLater_dist distLater_zero
 
 theorem Contractive.succ [OFE α] [OFE β] (f : α → β) [Contractive f] {n x y}
     (h : x ≡{n}≡ y) : f x ≡{n.succ}≡ f y :=
   Contractive.distLater_dist (distLater_succ.2 h)
 
+/-- A contractive function is non-expansive. -/
+instance [OFE α] [OFE β] (f : α → β) [Contractive f] : NonExpansive f where
+  ne := fun _ _ _ h => Contractive.distLater_dist (Dist.distLater h)
+
+/-- A contractive function preserves equivalence. -/
+theorem Contractive.eqv [OFE α] [OFE β] (f : α → β) [Contractive f] ⦃x y : α⦄ (h : x ≡ y) :
+    f x ≡ f y := NonExpansive.eqv h
+
+/-- Constant functions are contractive. -/
+instance [OFE α] [OFE β] {x : β} : Contractive (fun _ : α => x) where
+  distLater_dist := fun _ => Dist.rfl
+
+/-- The discrete OFE obtained from an equivalence relation `Equiv` -/
 def ofDiscrete (Equiv : α → α → Prop) (equiv_eqv : Equivalence Equiv) : OFE α where
   Equiv := Equiv
   Dist _ := Equiv
@@ -100,24 +123,41 @@ def ofDiscrete (Equiv : α → α → Prop) (equiv_eqv : Equivalence Equiv) : OF
   equiv_dist := (forall_const _).symm
   dist_lt h _ := h
 
+/-- A discrete OFE is one where equivalence is implied by `0`-equivalence. -/
 class Discrete (α : Type _) [OFE α] : Prop where
   discrete_0 {x y : α} : x ≡{0}≡ y → x ≡ y
 
+/-- For discrete OFEs, `n`-equivalence implies equivalence for any `n`. -/
+theorem Discrete.discrete_n [OFE α] [Discrete α] {n} {x y : α} (h : x ≡{n}≡ y) : x ≡ y :=
+  Discrete.discrete_0 (OFE.Dist.le h (Nat.zero_le _))
+
+/-- A morphism between OFEs, written `α -n> β`, is defined to be a function that is non-expansive. -/
 @[ext] structure Hom (α β : Type _) [OFE α] [OFE β] where
   f : α → β
   ne : NonExpansive f
 
+@[inherit_doc]
 infixr:25 " -n> " => Hom
 
 instance [OFE α] [OFE β] : CoeFun (α -n> β) (fun _ => α → β) := ⟨Hom.f⟩
+instance [OFE α] [OFE β] (f : α -n> β) : NonExpansive f := f.ne
 
+/-- The identity morphism on an OFE. -/
 protected def Hom.id [OFE α] : α -n> α where
   f := id
   ne.ne _ _ _ := id
 
+/-- The composition of two morphisms between OFEs. -/
 protected def Hom.comp [OFE α] [OFE β] [OFE γ] (g : β -n> γ) (f : α -n> β) : α -n> γ where
   f := g.f ∘ f.f
   ne.1 _ _ _ h := g.ne.1 (f.ne.1 h)
+
+@[simp] theorem Hom.id_apply [OFE α] {x} : (Hom.id : α -n> α) x = x := rfl
+@[simp] theorem Hom.comp_apply [OFE α] [OFE β] [OFE γ] {g : β -n> γ} {f : α -n> β} {x} :
+    (g.comp f) x = g (f x) := rfl
+
+@[simp] theorem Hom.id_comp [OFE α] [OFE β] {f : α -n> β} : Hom.id.comp f = f := rfl
+@[simp] theorem Hom.comp_id [OFE α] [OFE β] {f : α -n> β} : f.comp Hom.id = f := rfl
 
 theorem Hom.comp_assoc [OFE α] [OFE β] [OFE γ] [OFE δ]
     (h : γ -n> δ) (g : β -n> γ) (f : α -n> β) : (h.comp g).comp f = h.comp (g.comp f) := rfl
@@ -190,16 +230,81 @@ instance [OFE α] [OFE β] : OFE (α × β) where
   equiv_dist {_ _} := by simp [equiv_dist, forall_and]
   dist_lt h1 h2 := ⟨dist_lt h1.1 h2, dist_lt h1.2 h2⟩
 
+/-- An isomorphism between two OFEs is a pair of morphisms whose composition is equivalent to the identity morphism. -/
 @[ext] structure Iso (α β : Type _) [OFE α] [OFE β] where
   hom : α -n> β
   inv : β -n> α
   hom_inv : hom (inv x) ≡ x
   inv_hom : inv (hom x) ≡ x
 
+attribute [simp] Iso.hom_inv Iso.inv_hom
+
 instance [OFE α] [OFE β] : CoeFun (Iso α β) (fun _ => α -n> β) := ⟨Iso.hom⟩
+instance [OFE α] [OFE β] (iso : Iso α β) : NonExpansive iso.hom := iso.hom.ne
+instance [OFE α] [OFE β] (iso : Iso α β) : NonExpansive iso.inv := iso.inv.ne
+
+@[simp] theorem Iso.hom_inv_dist [OFE α] [OFE β] (iso : Iso α β) {n} {x} :
+    iso.hom (iso.inv x) ≡{n}≡ x :=
+  OFE.equiv_dist.mp (Iso.hom_inv iso) _
+
+@[simp] theorem Iso.inv_hom_dist [OFE α] [OFE β] (iso : Iso α β) {n} {x} :
+    iso.inv (iso.hom x) ≡{n}≡ x :=
+  OFE.equiv_dist.mp (Iso.inv_hom iso) _
+
+/-- OFE isomorphisms preserve equivalence. -/
+theorem Iso.hom_eqv [OFE α] [OFE β] (iso : Iso α β) ⦃x y⦄ :
+    x ≡ y ↔ iso.hom x ≡ iso.hom y :=
+  ⟨fun h => NonExpansive.eqv h,
+  fun h => Equiv.trans (Equiv.symm iso.inv_hom) <| Equiv.trans (NonExpansive.eqv h) (iso.inv_hom)⟩
+
+/-- The inverse of an OFE isomorphism preserves equivalence. -/
+theorem Iso.inv_eqv [OFE α] [OFE β] (iso : Iso α β) ⦃x y⦄ :
+    x ≡ y ↔ iso.inv x ≡ iso.inv y :=
+  ⟨fun h => NonExpansive.eqv h,
+  fun h => Equiv.trans (Equiv.symm iso.hom_inv) <| Equiv.trans (NonExpansive.eqv h) (iso.hom_inv)⟩
+
+/-- OFE isomorphisms preserve `n`-equivalence. -/
+theorem Iso.hom_dist [OFE α] [OFE β] (iso : Iso α β) {n} ⦃x y⦄ :
+    x ≡{n}≡ y ↔ iso.hom x ≡{n}≡ iso.hom y :=
+  ⟨fun h => NonExpansive.ne h, fun h => Dist.trans (Dist.symm iso.inv_hom_dist) <|
+    Dist.trans (NonExpansive.ne h) (iso.inv_hom_dist)⟩
+
+/-- The inverse of an OFE isomorphism preserves `n`-equivalence. -/
+theorem Iso.inv_dist [OFE α] [OFE β] (iso : Iso α β) {n} ⦃x y⦄ :
+    x ≡{n}≡ y ↔ iso.inv x ≡{n}≡ iso.inv y :=
+  ⟨fun h => NonExpansive.ne h, fun h => Dist.trans (Dist.symm iso.hom_inv_dist) <|
+    Dist.trans (NonExpansive.ne h) (iso.hom_inv_dist)⟩
+
+/-- The identity OFE isomorphism -/
+def Iso.id [OFE α] : Iso α α where
+  hom := Hom.id
+  inv := Hom.id
+  hom_inv := by intro x; simp
+  inv_hom := by intro x; simp
+
+@[simp] theorem Iso.id_apply [OFE α] {x} : ((Iso.id : Iso α α) : α -n> α) x = x := rfl
+
+/-- The inverse of an OFE isomorphism -/
+def Iso.symm [OFE α] [OFE β] (iso : Iso α β) : Iso β α where
+  hom := iso.inv
+  inv := iso.hom
+  hom_inv := by intro x; simp
+  inv_hom := by intro x; simp
+
+/-- Composition of OFE isomorphisms -/
+def Iso.comp [OFE α] [OFE β] [OFE γ] (iso1 : Iso β γ) (iso2 : Iso α β) : Iso α γ where
+  hom := iso1.hom.comp iso2.hom
+  inv := iso2.inv.comp iso1.inv
+  hom_inv := by
+    intro x; simp
+    exact .trans (NonExpansive.eqv <| .trans iso2.hom_inv .rfl) iso1.hom_inv
+  inv_hom := by
+    intro x; simp
+    exact .trans (NonExpansive.eqv <| .trans iso1.inv_hom .rfl) iso2.inv_hom
 
 end OFE
 
+/-- A chain in an OFE is a `Nat`-indexed sequence of elements that is upward-closed in terms of `n`-equivalence. -/
 structure Chain (α : Type _) [OFE α] where
   chain : Nat → α
   cauchy : n ≤ i → chain i ≡{n}≡ chain n
@@ -208,9 +313,27 @@ instance [OFE α] : CoeFun (Chain α) (fun _ => Nat → α) := ⟨Chain.chain⟩
 
 namespace Chain
 
+/-- The constant chain. -/
+def const [OFE α] (a : α) : Chain α where
+  chain := fun _ => a
+  cauchy _ := OFE.Dist.rfl
+
+@[simp] theorem const_apply [OFE α] {a : α} {n} : const a n = a := rfl
+
+/-- Mapping a chain through a non-expansive function. -/
 def map [OFE α] [OFE β] (f : α -n> β) (c : Chain α) : Chain β where
   chain n := f (c n)
   cauchy h := f.ne.1 (c.cauchy h)
+
+@[simp] theorem map_apply [OFE α] [OFE β] {f : α -n> β} {c : Chain α} {n} :
+    map f c n = f (c n) := rfl
+
+@[simp] theorem map_id [OFE α] {c : Chain α} : map (Hom.id : α -n> α) c = c := by
+  simp [map]
+
+theorem map_comp [OFE α] [OFE β] [OFE γ] {f : α -n> β} {g : β -n> γ} {c : Chain α} :
+    map (g.comp f) c = map g (map f c) := by
+  simp [map]
 
 end Chain
 
@@ -228,6 +351,21 @@ export IsCOFE (compl conv_compl)
 theorem conv_compl' [COFE α] {c : Chain α} {n i} (h : n ≤ i) : compl c ≡{n}≡ c i :=
   conv_compl.trans (c.cauchy h).symm
 
+/-- Chain maps commute with completion. -/
+theorem compl_map [COFE α] [COFE β] (f : α -n> β) (c : Chain α) :
+    compl (Chain.map f c) ≡ f (compl c) := by
+  refine OFE.equiv_dist.mpr (fun n => ?_)
+  exact Dist.trans conv_compl (NonExpansive.ne (Dist.symm conv_compl))
+
+/-- Constant chains complete to their constant value -/
+@[simp] theorem compl_const [COFE α] (a : α) : compl (Chain.const a) ≡ a :=
+  OFE.equiv_dist.mpr (fun _ => conv_compl)
+
+/-- Completion of discrete COFEs is the constant value. -/
+@[simp] theorem discrete_cofe_compl [COFE α] [OFE.Discrete α] (c : Chain α) : compl c ≡ c 0 :=
+  Discrete.discrete_0 conv_compl
+
+/-- The discrete COFE obtained from an equivalence relation `Equiv` -/
 def ofDiscrete (Equiv : α → α → Prop) (equiv_eqv : Equivalence Equiv) : COFE α :=
   let _ := OFE.ofDiscrete Equiv equiv_eqv
   { compl := fun c => c 0
