src/Iris/Std/Try.lean
@@ -4,5 +4,9 @@ Released under Apache 2.0 license as described in the file LICENSE.
 Authors: Mario Carneiro
 -/
 
+namespace Iris.ProofMode
+
 def try? [Monad m] [MonadExcept ε m] (x : m α) : m (Option α) :=
   try pure (some (← x)) catch _ => pure none
+
+end Iris.ProofMode
